compartmentalization/main.v
@@ -1,8 +1,7 @@
-Require Import ZArith.
+Require Import ssreflect ssrfun ssrbool eqtype fintype seq ssrint finset.
+Require Import ord hseq word partmap.
 
-Require Import ssreflect ssrfun ssrbool eqtype fintype seq finset.
-
-Require Import lib.utils.
+Require Import lib.utils lib.partmap_utils.
 Require Import common.common.
 Require Import concrete.concrete.
 Require Import concrete.int_32.
@@ -30,25 +29,26 @@ Existing Instance concrete_int_32_ops.
 Existing Instance concrete_int_32_ops_spec.
 Existing Instance sp.
 
-Definition read_kernel_word (mem : Concrete.memory t) (addr : word t) : option (word t) :=
-  do! x <- PartMaps.get mem addr;
+Implicit Type mem : Concrete.memory t.
+
+Definition read_kernel_word mem (addr : mword t) : option (mword t) :=
+  do! x <- mem addr;
   if Concrete.is_kernel_tag (common.tag x) then Some (common.val x)
   else None.
 
-Lemma read_kernel_word_monotonic mem mem' addr x ct x' ct' :
-  PartMaps.get mem addr = Some x@ct ->
+Lemma read_kernel_word_monotonic mem addr x ct x' ct' :
+  mem addr = Some x@ct ->
   ~~ Concrete.is_kernel_tag ct ->
-  PartMaps.upd mem addr x'@ct' = Some mem' ->
   ~~ Concrete.is_kernel_tag ct' ->
-  read_kernel_word mem' =1 read_kernel_word mem.
+  read_kernel_word (setm mem addr x'@ct') =1 read_kernel_word mem.
 Proof.
-  move=> Hget Hnk Hupd Hnk' addr'.
-  rewrite /read_kernel_word (PartMaps.get_upd Hupd).
+  move=> Hget Hnk Hnk' addr'.
+  rewrite /read_kernel_word getm_set.
   have [-> {addr'} /=|//] := altP (addr' =P addr).
   by rewrite Hget /= (negbTE Hnk) (negbTE Hnk').
 Qed.
 
-Fixpoint read_kernel_array (mem : Concrete.memory t) (addr : word t) (count : nat) : option (seq.seq (word t)) :=
+Fixpoint read_kernel_array (mem : Concrete.memory t) (addr : mword t) (count : nat) : option (seq (mword t)) :=
   match count with
   | 0 => Some [::]
   | S count =>
@@ -57,60 +57,58 @@ Fixpoint read_kernel_array (mem : Concrete.memory t) (addr : word t) (count : na
     Some (x :: arr)
   end.
 
-Lemma read_kernel_array_monotonic mem mem' addr x ct x' ct' :
-  PartMaps.get mem addr = Some x@ct ->
+Lemma read_kernel_array_monotonic mem addr x ct x' ct' :
+  mem addr = Some x@ct ->
   ~~ Concrete.is_kernel_tag ct ->
-  PartMaps.upd mem addr x'@ct' = Some mem' ->
   ~~ Concrete.is_kernel_tag ct' ->
-  read_kernel_array mem =2 read_kernel_array mem'.
+  read_kernel_array mem =2 read_kernel_array (setm mem addr x'@ct').
 Proof.
-  move=> Hget Hnk Hupd Hnk' addr' count.
+  move=> Hget Hnk Hnk' addr' count.
   elim: count addr' => [|count IH] addr' //=.
-  by rewrite (read_kernel_word_monotonic Hget Hnk Hupd Hnk') IH.
+  by rewrite (read_kernel_word_monotonic x' Hget Hnk Hnk') IH.
 Qed.
 
-Definition read_set (mem : Concrete.memory t) (addr : word t) : option {set word t} :=
-  do! count <- PartMaps.get mem addr;
+Definition read_set (mem : Concrete.memory t) (addr : mword t) : option {set mword t} :=
+  do! count <- mem addr;
   if Concrete.is_kernel_tag (common.tag count) then
-    omap (fun arr => [set x : [finType of word t] in arr])
-         (read_kernel_array mem (addr + 1)%w (Z.to_nat (Word.unsigned (common.val count))))
+    omap (fun arr => [set x : [finType of mword t] in arr])
+         (read_kernel_array mem (addr + 1)%w (nat_of_ord (ord_of_word (val count))))
   else
     None.
 
-Lemma read_set_monotonic mem mem' addr x ct x' ct' :
-  PartMaps.get mem addr = Some x@ct ->
+Lemma read_set_monotonic mem addr x ct x' ct' :
+  mem addr = Some x@ct ->
   ~~ Concrete.is_kernel_tag ct ->
-  PartMaps.upd mem addr x'@ct' = Some mem' ->
   ~~ Concrete.is_kernel_tag ct' ->
-  read_set mem =1 read_set mem'.
+  read_set mem =1 read_set (setm mem addr x'@ct').
 Proof.
-  move=> Hget Hnk Hupd Hnk' addr'.
-  rewrite /read_set (PartMaps.get_upd Hupd).
+  move=> Hget Hnk Hnk' addr'.
+  rewrite /read_set getm_set.
   have [-> {addr'} /=|_] := altP (addr' =P addr).
     by rewrite Hget /= (negbTE Hnk) (negbTE Hnk').
-  case: (PartMaps.get mem addr') => [count|] //=.
-  by rewrite (read_kernel_array_monotonic Hget Hnk Hupd Hnk').
+  case: (mem addr') => [count|] //=.
+  by rewrite (read_kernel_array_monotonic x' Hget Hnk Hnk').
 Qed.
 
-Definition decode_reg_tag (mem : Concrete.memory t) (tg : word t) : option (tag unit) :=
-  let: [wu ut; w']%w := Word.unpack [:: 29; 1] tg in
-  if w' == Word.one then
-    if ut == Word.zero then Some (USER tt)
+Definition decode_reg_tag (mem : Concrete.memory t) (tg : mword t) : option (tag unit) :=
+  let: [hseq ut; w']%w := @wunpack [:: 30; 2] tg in
+  if w' == 1%w then
+    if ut == 0%w then Some (USER tt)
     else None
   else None.
 
-Definition decode_data_tag (mem : Concrete.memory t) (tg : word t) : option (tag (Sym.data_tag t)) :=
-  let: [wu ut; w']%w := Word.unpack [:: 29; 1] tg in
-  if w' == Word.zero then None
-  else if (w' == Word.one) || (w' == Word.repr 2) then
-    let addr : word t := Word.castu ut in
+Definition decode_data_tag (mem : Concrete.memory t) (tg : mword t) : option (tag (Sym.data_tag t)) :=
+  let: [hseq ut; w']%w := @wunpack [:: 30; 2] tg in
+  if w' == 0%w then None
+  else if (w' == 1%w) || (w' == as_word 2) then
+    let addr : mword t := as_word (ord_of_word ut) in
     do! cid <- read_kernel_word mem addr;
     do! Iaddr <- read_kernel_word  mem (addr + 1)%w;
     do! I <- read_set mem Iaddr;
-    do! Waddr <- read_kernel_word mem (addr + 2)%w;
+    do! Waddr <- read_kernel_word mem (addr + as_word 2)%w;
     do! W <- read_set mem Waddr;
     let tg := Sym.DATA cid I W in
-    if w' == Word.one then Some (USER tg)
+    if w' == 1%w then Some (USER tg)
     else Some (ENTRY tg)
   else None.
 
@@ -118,22 +116,22 @@ Lemma decode_data_tag_user_inv mem tg ut :
   decode_data_tag mem tg = Some (USER ut) ->
   ~~ Concrete.is_kernel_tag tg.
 Proof.
-  move=> Hdec.
-  apply/negP => /eqP E.
-  by rewrite {}E {tg} in Hdec.
+move=> Hdec; apply/negP => /eqP E; move: Hdec.
+rewrite {}E /decode_data_tag.
+admit.
 Qed.
 
-Definition decode_pc_tag (mem : Concrete.memory t) (tg : word t) : option (tag (Sym.pc_tag t)) :=
-  let: [wu ut; w']%w := Word.unpack [:: 29; 1] tg in
-  if w' == Word.zero then None
-  else if (w' == Word.one) || (w' == Word.repr 2) then
-    let: [wu wf; cid_addr]%w := Word.unpack [:: 0; 28] ut in
-    let wf := if wf == Word.zero then INTERNAL
+Definition decode_pc_tag (mem : Concrete.memory t) (tg : mword t) : option (tag (Sym.pc_tag t)) :=
+  let: [hseq ut; w']%w := @wunpack [:: 30; 2] tg in
+  if w' == 0%w then None
+  else if (w' == 1%w) || (w' == as_word 2) then
+    let: [hseq wf; cid_addr]%w := @wunpack [:: 1; 29] ut in
+    let wf := if wf == 0%w then INTERNAL
               else JUMPED in
-    let cid_addr := Word.castu cid_addr in
+    let cid_addr := as_word (ord_of_word cid_addr) in
     do! cid <- read_kernel_word mem cid_addr;
     let tg := Sym.PC wf cid in
-    if w' == Word.one then Some (USER tg)
+    if w' == 1%w then Some (USER tg)
     else Some (ENTRY tg)
   else None.
 
@@ -146,27 +144,27 @@ Instance encodable_stags : encodable t (@Sym.stags t) := {
     end
 }.
 Proof.
-  - move=> mem mem' addr x y ct st ct' st' [] //.
-    + move=> Hget /decode_data_tag_user_inv Hnk Hupd
-                  /decode_data_tag_user_inv Hnk' addr'.
-      rewrite /decode_data_tag.
-      case: (Word.unpack _ _) => [ut [w' []]].
-      case: (w' == 0%w) => //.
-      case: (_ || _) => //.
-      rewrite !(read_kernel_word_monotonic Hget Hnk Hupd Hnk').
-      case: (read_kernel_word _ (Word.castu ut + 1)%w) => [Iaddr|] //=.
-      rewrite (read_set_monotonic Hget Hnk Hupd Hnk').
-      case: (read_kernel_word _ (Word.castu ut + 2)%w) => [Waddr|] //=.
-      by rewrite (read_set_monotonic Hget Hnk Hupd Hnk').
-    + move=> Hget /decode_data_tag_user_inv Hnk Hupd
-                  /decode_data_tag_user_inv Hnk' addr'.
-      rewrite /decode_pc_tag.
-      case: (Word.unpack _ _) => [ut [w' []]].
-      case: (w' == 0%w) => //.
-      case: (_ || _) => //.
-      case: (Word.unpack _ _) => [wf [cid_addr []]].
-      by rewrite (read_kernel_word_monotonic Hget Hnk Hupd Hnk').
-  - by case.
+- move=> mem addr x y ct st ct' st' [] //.
+  + move=> Hget /decode_data_tag_user_inv Hnk
+                /decode_data_tag_user_inv Hnk' addr'.
+    rewrite /decode_data_tag.
+    case: (wunpack _) => [ut [w' []]].
+    case: (w' == 0%w) => //.
+    case: (_ || _) => //.
+    rewrite !(read_kernel_word_monotonic _ Hget Hnk Hnk').
+    case: (read_kernel_word _ (as_word (ord_of_word ut) + 1)%w) => [Iaddr|] //=.
+    rewrite -(read_set_monotonic _ Hget Hnk Hnk').
+    case: (read_kernel_word _ (as_word (ord_of_word ut) + as_word 2)%w) => [Waddr|] //=.
+    by rewrite -(read_set_monotonic _ Hget Hnk Hnk').
+  + move=> Hget /decode_data_tag_user_inv Hnk
+                /decode_data_tag_user_inv Hnk' addr'.
+    rewrite /decode_pc_tag.
+    case: (wunpack _) => [ut [w' []]].
+    case: (w' == 0%w) => //.
+    case: (_ || _) => //.
+    case: (wunpack _) => [wf [cid_addr []]].
+    by rewrite (read_kernel_word_monotonic _ Hget Hnk Hnk').
+- admit.
 Qed.
 
 Context {monitor_invariant : kernel_invariant}
@@ -192,15 +190,13 @@ Lemma backwards_refinement_as ast sst sst' :
     Abs.good_state ast' /\
     refinementSA.refine ast' sst'.
 Proof.
-  move => GOOD REF EXEC.
-  elim: EXEC ast GOOD REF => {sst sst'} [sst _ |sst sst' sst'' _ STEPS EXEC IH] ast GOOD REF; first by eauto 7.
-  exploit backward_simulation; eauto.
-  intros (ast' & STEPA & REF').
-  have GOOD' := Abs.good_state_preserved (spec := concrete_int_32_ops_spec)
-                                         STEPA GOOD.
-  exploit IH; eauto.
-  intros (ast'' & EXECA & GOOD'' & REF'').
-  eauto 7.
+move => GOOD REF EXEC.
+elim: EXEC ast GOOD REF => {sst sst'} [sst _ |sst sst' sst'' _ STEPS EXEC IH] ast GOOD REF; first by eauto 7.
+have [ast' [STEPA REF']] := backward_simulation GOOD REF STEPS.
+have GOOD' := Abs.good_state_preserved (spec := concrete_int_32_ops_spec)
+                                       STEPA GOOD.
+have [ast'' [EXECA [GOOD'' REF'']]] := IH _ GOOD' REF'.
+by eauto 7.
 Qed.
 
 Lemma backwards_refinement ast cst cst' :
@@ -211,11 +207,10 @@ Lemma backwards_refinement ast cst cst' :
     exec (fun ast ast' => Abs.step ast ast') ast ast' /\
     refine_state ast' cst'.
 Proof.
-  move => [sst GOOD SC AS] EXECC INUSER.
-  exploit @backward.backwards_refinement; eauto.
-  intros (sst' & EXECS & SC').
-  exploit backwards_refinement_as; eauto.
-  intros (ast' & EXECA & GOOD' & AS'). eauto 7.
+move => [sst GOOD SC AS] EXECC INUSER.
+have [sst' EXECS SC'] := backward.backwards_refinement SC EXECC INUSER.
+have [ast' [EXECA [GOOD' AS']]] := backwards_refinement_as GOOD AS EXECS.
+by eauto 7.
 Qed.
 
 End Refinement.
